src/program_logic/crash_inv.v
@@ -82,6 +82,33 @@ Proof.
   - iIntros. rewrite difference_diag_L. iModIntro; eauto.
 Qed.
 
+Lemma wpc_crash_inv_open_modify Qnew s k k' E1 E1' E2 e Φ Φc Q P N γ :
+  E1 ⊆ E1' →
+  ↑N ⊆ E1 →
+  S k < k' →
+  to_val e = None →
+  crash_inv_full N (LVL k') E1' γ Q P -∗
+  (Φc ∧ (Q -∗ WPC e @ NotStuck; (LVL k); (E1 ∖ ↑N); ∅
+                    {{λ v, Qnew v ∗ □ (Qnew v -∗ P)  ∗ (crash_inv_full N (LVL k') E1' γ (Qnew v) P -∗ (Φ v ∧ Φc))}}
+                    {{ Φc ∗ P }})) -∗
+  WPC e @ s; LVL (S (S k)); E1; E2 {{ Φ }} {{ Φc }}.
+Proof.
+  iIntros (????) "Hfull Hwp".
+  iDestruct "Hfull" as (??) "(#Hinv&Hval&#Hwand)".
+  iApply (wpc_staged_inv_open _ _ _ _ _ _ _ _ _ _ _ Qnew); eauto.
+  iFrame "Hinv". iFrame.
+  iSplit.
+  { iDestruct "Hwp" as "($&_)". }
+  iDestruct "Hwp" as "(_&Hwp)".
+  iIntros "HQ". iSpecialize ("Hwp" with "HQ").
+  iApply (wpc_strong_mono' with "Hwp"); eauto.
+  iSplit.
+  - iIntros (?) "(HQ&#Hwand'&HQrest)".
+    iModIntro. iFrame "HQ Hwand'". iIntros "Hval".
+    iApply "HQrest". iExists _, _. iFrame. iFrame "Hinv". iFrame "Hwand'".
+  - iIntros. rewrite difference_diag_L. iModIntro; eauto.
+Qed.
+
 Lemma wpc_crash_inv_init s k k' N E1 E2 e Φ Φc P γ :
   k' < k →
   ↑N ⊆ E1 →
@@ -94,12 +121,12 @@ Proof.
   iApply wpc_staged_inv_init; last (by iFrame); eauto.
 Qed.
 
-Lemma crash_inv_open N k E E1 γ P Q R:
+Lemma crash_inv_open N k' k E E' E1 γ P Q R:
   ↑N ⊆ E →
-  crash_inv_full N k E1 γ Q P -∗
-  ((Q ∗ (▷ Q ={E∖↑N,E}=∗ crash_inv_full N k E1 γ Q P)) ∨ (C ∗ |={E∖↑N, E}=> emp)
-   -∗ |={E ∖ ↑N, E}_k=> R) -∗
-  (|={E,E}_(S (S k))=> R).
+  crash_inv_full N k' E1 γ Q P -∗
+  ((Q ∗ (▷ Q ={E∖↑N,E}=∗ crash_inv_full N k' E1 γ Q P)) ∨ (C ∗ |={E∖↑N, E}=> emp)
+   -∗ |={E ∖ ↑N, E'}_k=> R) -∗
+  (|={E,E'}_(S (S k))=> R).
 Proof.
   iIntros (?) "H Hwp".
   iDestruct "H" as (??) "(#Hinv&H&#Hwand)".
@@ -116,6 +143,31 @@ Proof.
     { iFrame. iAlways. iIntros. iApply step_fupdN_inner_later; auto. iNext.
       iDestruct ("Hwand" with "[$]") as "$". }
     iModIntro. iExists _, _. iFrame "H Hinv Hwand".
+  - iRight. iFrame.
+Qed.
+
+Lemma crash_inv_open_modify N k' k E E' E1 γ P Q R:
+  ↑N ⊆ E →
+  crash_inv_full N k' E1 γ Q P -∗
+  ((Q ∗ (∀ Q', ▷ Q' ∗ □ (Q' -∗ P) ={E∖↑N,E}=∗ crash_inv_full N k' E1 γ Q' P)) ∨ (C ∗ |={E∖↑N, E}=> emp)
+   -∗ |={E ∖ ↑N, E'}_k=> R) -∗
+  (|={E,E'}_(S (S k))=> R).
+Proof.
+  iIntros (?) "H Hwp".
+  iDestruct "H" as (??) "(#Hinv&H&#Hwand)".
+  iMod (staged_inv_open with "[H]") as "HQ"; try iFrame "H Hinv"; eauto.
+  iMod (fupd_intro_mask' _ ∅) as "Hclo"; first set_solver.
+  iModIntro.
+  rewrite Nat_iter_S.
+  iModIntro. iNext. iModIntro.
+  rewrite Nat_iter_S.
+  iModIntro. iNext. iMod "Hclo" as "_".
+  iApply ("Hwp" with "[HQ]").
+  iDestruct "HQ" as "[(HQ&Hclo)|(?&HC&?)]".
+  - iLeft. iFrame. iIntros (Q') "(HQ'&#Hwand')". iMod ("Hclo" $! Q' True%I with "[HQ']") as "H".
+    { iFrame. iAlways. iIntros. iApply step_fupdN_inner_later; auto. iNext.
+      iDestruct ("Hwand'" with "[$]") as "$". }
+    iModIntro. iExists _, _. iFrame "H Hinv Hwand'".
   - iRight. iFrame.
 Qed.
 
